stupid bug

src/certigrad/aevb/grads_correct.lean
@@ -30,7 +30,7 @@ do to_expr ```((g a x_data)^.targets ⊆ env.keys (fdict a ws x_data)) >>= asser
 
 private meta def prove_dep_hyps (tgt : expr) : tactic unit :=
 do to_expr ```(well_formed_at (g a x_data)^.costs (g a x_data)^.nodes (fdict a ws x_data) %%tgt) >>= assert `H_wf,
-     solve1 (constructor >> all_goals cgsimp),
+     focus1 (constructor >> all_goals cgsimp), rotate 1,
    to_expr ```(grads_exist_at (g a x_data)^.nodes (fdict a ws x_data) %%tgt) >>= assert `H_gs_exist,
      solve1 (cgsimp),
    to_expr ```(is_gintegrable (λ m, ⟦compute_grad_slow (g a x_data)^.costs (g a x_data)^.nodes m %%tgt⟧) (fdict a ws x_data) (g a x_data)^.nodes dvec.head) >>= assert `H_gint,
@@ -48,33 +48,34 @@ tac_base <|>
 private meta def prove_aevb_base : tactic unit :=
 do exfalso,
    H_at_idx ← get_local `H_at_idx,
-   to_expr ```(list.at_idx_over H_at_idx dec_trivial) >>= exact
+   to_expr ```(list.at_idx_over %%H_at_idx dec_trivial) >>= exact
 
 private meta def prove_aevb_step : tactic unit :=
 do H_at_idx ← get_local `H_at_idx,
-   H ← mk_app `and.right [H_at_idx],
-   rewrite_core reducible tt tt occurrences.all ff H,
-   H_type ← infer_type H,
-   (tgt, new_tgt) ← match_eq H_type,
+   mk_app `and.right [H_at_idx] >>= note `H_tgt_eq,
+   H_tgt_eq_type ← get_local `H_tgt_eq >>= infer_type,
+   s ← join_user_simp_lemmas true [`cgsimp],
+   (H_tgt_eq_new_type, pr) ← simplify s H_tgt_eq_type {},
+   get_local `H_tgt_eq >>= λ H_tgt_eq, replace_hyp H_tgt_eq H_tgt_eq_new_type pr,
+   get_local `H_tgt_eq >>= subst,
+   (tgt, new_tgt) ← match_eq H_tgt_eq_new_type,
    prove_dep_hyps new_tgt,
-   to_expr ```(backprop_correct (fdict a ws x_data) (g a x_data)^.targets H_tgts_ss_inputs H_at_idx H_wf H_gs_exist H_gint H_can_diff) >>= exact
+   to_expr ```(backprop_correct (fdict a ws x_data) (g a x_data)^.targets H_tgts_ss_inputs H_at_idx H_wf H_gs_exist H_pdfs_exist H_gint H_can_diff) >>= exact
 
 meta def prove_aevb_ok : tactic unit :=
 do -- introduce hypotheses
-   [tgt, idx, H_at_idx] ← intros | failed,
+   [tgt, idx, H_at_idx] ← intros | fail "can't intro hyps",
    -- prove independent hyps once and for all
    prove_indep_hyps,
    -- repeated case-analysis on idx
    forall_idxs prove_aevb_base prove_aevb_step idx
 
-lemma aevb_backprop_correct (a : arch) (ws : weights a) (x_data : T [a^.n_in, a^.n_x]) :
+lemma aevb_backprop_correct :
 ∀ (tgt : reference) (idx : ℕ) (H_at_idx : at_idx g^.targets idx tgt),
 ∇ (λ θ₀, E (graph.to_dist (λ m, ⟦sum_costs m g^.costs⟧) (env.insert tgt θ₀ fdict) g^.nodes) dvec.head) (env.get tgt fdict)
 =
 E (graph.to_dist (λ m, backprop g^.costs g^.nodes m g^.targets) fdict g^.nodes) (λ dict, dvec.get tgt.2 dict idx) :=
-begin
-prove_aevb_ok
-end
+by prove_aevb_ok
 
 end proof
 end aevb
